Heap.v
@@ -99,12 +99,6 @@ Definition update (h : heap) k v := M.add k v h.
 
 Definition empty : heap := M.empty Dynamic.
 
-Definition read {a : Type} (k : Addr.t) (h : heap) (H : exists v, M.MapsTo k (dyn a v) h) : a.
-Admitted.
-
-Definition readMaps {a : Type} (k : Addr.t) (v : a) (h : heap) (P : exists v, M.MapsTo k (dyn a v) h) (H : M.MapsTo k (dyn a v) h) : read k h P = v.
-Admitted.
-
 (** Allocation **)
 
 Fixpoint maxTree {e : Type} (t : M.Raw.tree e) (a : Addr.t) : Addr.t :=
